feat(tm): dsum, blang

src/tm.lean
@@ -1,5 +1,5 @@
 import tactic data.vector.basic data.vector.zip algebra.big_operators.basic algebra.big_operators.norm_num
-import vorspiel
+ vorspiel lencodable
 
 open_locale big_operators
 
@@ -15,7 +15,20 @@ inductive language (Γ : Type u)
 notation `␣` := language.blank 
 notation `␤` := language.start
 
-instance {Γ : Type u} : inhabited (language Γ) := ⟨␣⟩
+namespace language
+variables {Γ : Type u}
+
+instance : inhabited (language Γ) := ⟨␣⟩
+
+def language_equiv_option_sum_bool : language Γ ≃ bool ⊕ Γ :=
+{ to_fun := λ l, match l with | ␣ := sum.inl ff | ␤ := sum.inl tt | chr x := sum.inr x end,
+  inv_fun := λ l, match l with | (sum.inl ff) := ␣ | (sum.inl tt) := ␤ | sum.inr x := chr x end,
+  left_inv := λ l, by rcases l; simp; refl,
+  right_inv := λ l, by { rcases l; simp, { rcases l; refl }, refl } }
+
+instance [fintype Γ] : fintype (language Γ) := fintype.of_equiv (bool ⊕ Γ) language_equiv_option_sum_bool.symm
+
+end language
 
 class state_lang (Q : Type u) :=
 (start : Q)
@@ -38,17 +51,45 @@ inductive instruction
 | right : instruction
 | left  : instruction
 
-instance : inhabited instruction := ⟨instruction.stay⟩
+namespace instruction
 
-@[simp] def instruction.apply : instruction → ℕ → ℕ
-| instruction.stay  ι := ι
-| instruction.right ι := ι + 1
-| instruction.left  ι := ι - 1
+instance : inhabited instruction := ⟨stay⟩
 
-@[simp] lemma instruction.apply_default (n) : instruction.apply default n = n := rfl
+@[simp] def apply : instruction → ℕ → ℕ
+| stay  ι := ι
+| right ι := ι + 1
+| left  ι := ι - 1
 
-@[simp] lemma instruction.default_nth (ι : ℕ) (i) : (default : vector instruction ι).nth i = instruction.stay :=
+@[simp] lemma apply_default (n) : apply default n = n := rfl
+
+@[simp] lemma default_nth (ι : ℕ) (i) : (default : vector instruction ι).nth i = stay :=
 by { unfold default, simp }
+
+def equiv_unit_sums : instruction ≃ unit ⊕ unit ⊕ unit :=
+{ to_fun := λ i, match i with | stay := sum.inl () | right := sum.inr (sum.inl ()) | left := sum.inr (sum.inr ()) end,
+  inv_fun := λ i, match i with | sum.inl () := stay | sum.inr (sum.inl ()) := right | sum.inr (sum.inr ()) := left end,
+  left_inv := λ i, by rcases i; refl,
+  right_inv := λ i, by { rcases i; simp, rcases i, refl, rcases i; rcases i; refl } }
+
+instance : fintype instruction := fintype.of_equiv (unit ⊕ unit ⊕ unit) equiv_unit_sums.symm
+
+@[simp] lemma card : fintype.card instruction = 3 := by simpa using fintype.card_congr equiv_unit_sums
+
+variables {ι}
+
+def Stay : vector instruction ι := vector.repeat stay ι
+
+@[simp] lemma Stay_nth (i : fin ι) : Stay.nth i = stay := by simp[Stay]
+
+def Right : vector instruction ι := vector.repeat right ι
+
+@[simp] lemma Right_nth (i : fin ι) : Right.nth i = right := by simp[Right]
+
+def Left : vector instruction ι := vector.repeat left ι
+
+@[simp] lemma Left_nth (i : fin ι) : Left.nth i = left := by simp[Left]
+
+end instruction
 
 structure word :=
 (c : Q)
@@ -58,6 +99,29 @@ structure word :=
 (x : vector Γ ι)
 
 notation `⟮` c `, ` z `; ` u ` | ` q `, ` x `⟯`:80 := word.mk c z u q x
+
+namespace word
+
+def equiv_prod : word Γ Q ι ≃ Q × vector Γ ι × vector instruction ι × Q × vector Γ ι :=
+{ to_fun := λ w, match w with ⟮c, z; u | q, x⟯ := (c, z, u, q, x) end,
+  inv_fun := λ w, match w with (c, z, u, q, x) := ⟮c, z; u | q, x⟯ end,
+  left_inv := λ w, by rcases w; refl,
+  right_inv := λ w, by rcases w with ⟨_, w⟩; rcases w with ⟨_, w⟩; rcases w with ⟨_, w⟩; rcases w with ⟨_, w⟩; refl }
+
+open fintype
+
+instance [fintype Γ] [fintype Q] : fintype (word Γ Q ι) :=
+fintype.of_equiv (Q × vector Γ ι × vector instruction ι × Q × vector Γ ι) (equiv_prod _ _ _).symm
+
+lemma card [fintype Γ] [fintype Q] : card (word Γ Q ι) = card Q^2 * (3 * card Γ^2)^ι :=
+calc card (word Γ Q ι) = card Q * card Γ^ι * 3^ι * card Q * card Γ^ι
+  : by simpa[mul_assoc] using fintype.card_congr (equiv_prod Γ Q ι)
+                   ... = card Q * card Q * 3^ι * card Γ^ι * card Γ^ι
+  : by ring
+                   ... = card Q^2 * (3 * card Γ^2)^ι
+  : by simp[pow_two, mul_pow]; ring
+
+end word
 
 structure model :=
 (state : Q) 
@@ -74,7 +138,7 @@ namespace sentence
 variables {Γ Q ι}
 variables (σ : sentence Γ Q ι)
 
-instance : set_like (sentence Γ Q ι) (word Γ Q ι) := ⟨sentence.carrier,by { rintros ⟨_, _⟩ ⟨_, _⟩, simp }⟩
+instance : set_like (sentence Γ Q ι) (word Γ Q ι) := ⟨sentence.carrier, λ ⟨_, _⟩ ⟨_, _⟩, by simp⟩
 
 lemma mem_def (w : word Γ Q ι) : w ∈ σ ↔ w ∈ σ.carrier := iff.rfl
 
@@ -83,6 +147,16 @@ lemma proper {c z u q x} : ⟮c, z; u | q, x⟯ ∈ σ → q ≠ state_lang.halt
 @[simp] lemma start_notin (c z u x) : ⟮c, z; u | halt, x⟯ ∉ σ := λ A, by simpa using σ.proper A
 
 @[simp] lemma halt_notin (z u q x) : ⟮start, z; u | q, x⟯ ∉ σ := λ A, by simpa using σ.proper A 
+
+lemma carrier_finite [fintype Γ] [fintype Q] : σ.carrier.finite := set.to_finite _
+
+noncomputable instance [fintype Γ] [fintype Q] : fintype (sentence Γ Q ι) := fintype.of_injective carrier (λ ⟨_, _⟩ ⟨_, _⟩, by simp)
+
+def is_halt (q : Q) : Prop := ∀ ⦃c z u x⦄, ⟮c, z; u | q, x⟯ ∉ σ
+
+def is_start (c : Q) : Prop := ∀ ⦃z u x q⦄, ⟮c, z; u | q, x⟯ ∉ σ
+
+lemma coe_carrier : (σ : set (word Γ Q ι)) = σ.carrier := by refl
 
 end sentence
 
@@ -152,22 +226,26 @@ def sentence.deterministic (σ : sentence Γ Q ι) : Prop :=
 
 namespace sentence
 
-inductive of_fun_aux (δ : Q × vector Γ ι → option (Q × vector Γ ι × vector instruction ι)) : set (word Γ Q ι)
-| intro : ∀ {q x c z u}, δ ⟨q, x⟩ = some ⟨c, z, u⟩ → of_fun_aux ⟮c, z; u | q, x⟯
+inductive of_fun_aux (δ : Q → vector Γ ι → option (Q × vector Γ ι × vector instruction ι)) : set (word Γ Q ι)
+| intro : ∀ {q x c z u}, δ q x = some ⟨c, z, u⟩ → of_fun_aux ⟮c, z; u | q, x⟯
 
-def of_fun (δ : Q × vector Γ ι → option (Q × vector Γ ι × vector instruction ι))
-  (H : ∀ {q x c z u}, δ ⟨q, x⟩ = some ⟨c, z, u⟩ → q ≠ halt ∧ c ≠ start) : sentence Γ Q ι :=
+def of_fun (δ : Q → vector Γ ι → option (Q × vector Γ ι × vector instruction ι))
+  (H : ∀ {q x c z u}, δ q x = some ⟨c, z, u⟩ → q ≠ halt ∧ c ≠ start) : sentence Γ Q ι :=
 { carrier := of_fun_aux δ,
   proper' := λ c z u q x, by { rintro ⟨_, _, _, _, _, h⟩, exact H h } }
 
 namespace of_fun
-variables (δ : Q × vector Γ ι → option (Q × vector Γ ι × vector instruction ι))
+variables (δ : Q → vector Γ ι → option (Q × vector Γ ι × vector instruction ι))
 
 lemma carrier_eq {H} : (of_fun δ H).carrier = of_fun_aux δ := rfl
 
-@[simp] lemma mem_iff {H} {c z u q x} : ⟮c, z; u | q, x⟯ ∈ of_fun δ H ↔ δ ⟨q, x⟩ = some ⟨c, z, u⟩ :=
+@[simp] lemma mem_iff {H} {c z u q x} : ⟮c, z; u | q, x⟯ ∈ of_fun δ H ↔ δ q x = some ⟨c, z, u⟩ :=
 by { simp[sentence.mem_def], split,
   { rintros ⟨_, _, _, _, _, h⟩, exact h }, { intros h, exact of_fun_aux.intro h } }
+
+lemma none_is_halt {q H} : (of_fun δ H).is_halt q ↔ ∀ x, δ q x = none :=
+by { simp [is_halt, mem_iff, option.eq_none_iff_forall_not_mem], split,
+  { rintros h x c ⟨z, u⟩ eqn, exact h eqn }, { rintros h c z u x, exact h x c (z, u) } }
 
 lemma of_fn.deterministic {H} : deterministic (of_fun δ H) :=
 λ _ _ _ _ _ _ _ _, by { simp, intros h₁ h₂, simpa[h₁] using h₂ }
@@ -211,24 +289,18 @@ by { cases n, { simp at gt, contradiction },
 by { cases n, { simp at h, contradiction },
      { simp[tape_of], have : n ≥ x.length, exact nat.succ_le_succ_iff.mp h, exact nat.le_lt_antisymm this } }
 
-structure time_bounded_computable_by_NDTM (f : list Γ → list Γ) (T : ℕ → ℕ) :=
+structure fun_time_bounded_computable_by_NDTM (f : vector (list Γ) ι → vector (list Γ) ι) (T : ℕ → ℕ) :=
 (Q : Type*)
 (Q_fin : finite Q)
 (Q_state : state_lang Q)
-(σ : sentence (language Γ) Q ι.succ.succ)
-(reduction : ∀ (X : list Γ), 
-  model.is_halt_in_step σ (T X.length) (⟦start, tape_of X ::ᵥ default, default⟧) ∧
-  ⟦start, tape_of X ::ᵥ default, default⟧ ⟶^(≤ T X.length)[σ]↓ ⟦halt, vector.concat default (tape_of (f X)), default⟧)
+(σ : sentence (language Γ) Q ι)
+(reduction : ∀ (X : vector (list Γ) ι), 
+  model.is_halt_in_step σ (T X.length) (⟦start, X.map tape_of, default⟧) ∧
+  ⟦start, X.map tape_of, default⟧ ⟶^(≤ T X.length)[σ]↓ ⟦halt, (f X).map tape_of, default⟧)
 
-
-structure time_bounded_computable_by_TM (f : list Γ → list Γ) (T : ℕ → ℕ) :=
-(Q : Type*)
-(Q_fin : finite Q)
-(Q_state : state_lang Q)
-(σ : sentence (language Γ) Q ι.succ.succ)
+structure fun_time_bounded_computable_by_TM (f : vector (list Γ) ι → vector (list Γ) ι) (T : ℕ → ℕ)
+  extends fun_time_bounded_computable_by_NDTM f T :=
 (deterministic : σ.deterministic)
-(reduction : ∀ (X : list Γ), 
-  ⟦start, tape_of X ::ᵥ default, default⟧ ⟶^(≤ T X.length)[σ]↓ ⟦halt, vector.concat default (tape_of (f X)), default⟧)
 
 end TM
 
@@ -254,7 +326,7 @@ variables {m₁ m₂ m₃ : model Γ Q ι} {σ : sentence Γ Q ι}
 @[simp] lemma reduct_tape_read {T : vector (ℕ → Γ) ι} {H : vector ℕ ι} : reduct_tape T H (read T H) = T :=
 by { ext, simp, rintros rfl, refl }
 
-@[simp] lemma reduct_head_default {H : vector ℕ ι} : reduct_head H default = H :=
+@[simp] lemma reduct_head_Stay {H : vector ℕ ι} : reduct_head H instruction.Stay = H :=
 by { ext, simp, }
 
 lemma reduction.iff {q₁ q₂ : Q} {T₁ T₂ : vector (ℕ → Γ) ι} {H₁ H₂ : vector ℕ ι}  :
@@ -265,7 +337,9 @@ lemma reduction.iff {q₁ q₂ : Q} {T₁ T₂ : vector (ℕ → Γ) ι} {H₁ H
 
 @[simp] lemma time_bounded_reductions.refl {s} : m₁ ⟶^(≤ s)[σ] m₁ := power_le.refl
 
-@[simp] lemma time_reductions.refl : m₁ ⟶^(0)[σ] m₁ := power.zero _
+lemma time_reductions.refl : m₁ ⟶^(0)[σ] m₁ := power.zero _
+
+@[simp] lemma time_reductions_zero_iff : (m₁ ⟶^(0)[σ] m₂) ↔ m₁ = m₂ := power.zero_iff
 
 lemma time_bounded_reductions.of_le {s₁ s₂} (le : s₁ ≤ s₂) (h : m₁ ⟶^(≤ s₁)[σ] m₂) :
   m₁ ⟶^(≤ s₂)[σ] m₂ := power_le.of_le le h
@@ -341,46 +415,69 @@ namespace sentence
 variables {Q R} (q c : Q) (h : q ≠ halt ∧ c ≠ start) 
 
 inductive fix_q_aux : word Γ Q ι → Prop
-| intro : ∀ (z : vector Γ ι), fix_q_aux ⟮c, z; default | q, z⟯
+| intro : ∀ (z : vector Γ ι), fix_q_aux ⟮c, z; instruction.Stay | q, z⟯
 
 def fix_q (q c : Q) (h : q ≠ halt ∧ c ≠ start) : sentence Γ Q ι :=
 { carrier := fix_q_aux q c,
   proper' := λ c' z u q' x, by { rintros ⟨⟩, exact h } } 
 
 @[simp] lemma fix_q_mem (z : vector Γ ι) :
-  ⟮c, z; default | q, z⟯ ∈ (fix_q q c h : sentence Γ Q ι) :=
+  ⟮c, z; instruction.Stay | q, z⟯ ∈ (fix_q q c h : sentence Γ Q ι) :=
 fix_q_aux.intro _
+
+lemma fix_q_mem_iff {c z u q x q₁ q₂ h} :
+  ⟮c, z; u| q, x⟯ ∈ (fix_q q₁ q₂ h : sentence Γ Q ι) ↔ c = q₂ ∧ z = x ∧ q = q₁ ∧ u = instruction.Stay :=
+⟨by { rintros ⟨⟩, simp; refl }, by { rintros ⟨rfl, rfl, rfl, rfl⟩, exact fix_q_aux.intro _ }⟩
 
 lemma fix_q.deterministic : deterministic (fix_q q c h : sentence Γ Q ι) :=
 by { rintros q' x c₁ c₂ z₁ z₂ u₁ u₂ h₁ h₂, rcases h₁, rcases h₂, simp }
 
 @[simp] lemma fix_q_reduction (T : vector (ℕ → Γ) ι) (H : vector ℕ ι) : ⟦q, T, H⟧ ⟶¹[fix_q q c h] ⟦c, T, H⟧ :=
-reduction.iff.mpr ⟨read T H, default, by simp, by simp⟩
+reduction.iff.mpr ⟨read T H, instruction.Stay, by simp, by simp⟩
 
 instance : has_union (sentence Γ Q ι) := ⟨λ σ τ,
 { carrier := σ ∪ τ,
   proper' := by { rintros c z u q x (h | h), { exact σ.proper h }, { exact τ.proper h } } }⟩
 
 def deterministic.union {σ τ : sentence Γ Q ι} (d₁ : deterministic σ) (d₂ : deterministic τ) 
-  (h : ∀ {q x c₁ c₂ z₁ z₂ u₁ u₂}, ⟮c₁, z₁; u₁ | q, x⟯ ∈ σ → ⟮c₂, z₂; u₂ | q, x⟯ ∈ τ → c₁ = c₂ ∧ z₁ = z₂ ∧ u₁ = u₂) : deterministic (σ ∪ τ) :=
+  (h : ∀ {q x c₁ c₂ z₁ z₂ u₁ u₂}, ⟮c₁, z₁; u₁ | q, x⟯ ∈ σ → ⟮c₂, z₂; u₂ | q, x⟯ ∈ τ → c₁ = c₂ ∧ z₁ = z₂ ∧ u₁ = u₂) :
+  deterministic (σ ∪ τ) :=
 begin
   rintros q x c₁ c₂ z₁ z₂ u₁ u₂ (h₁ | h₁) (h₂ | h₂),
   { exact d₁ h₁ h₂ }, { exact h h₁ h₂ }, { simp [h h₂ h₁] }, { exact d₂ h₁ h₂ }
 end
 
-def dsum_suml (σ : sentence Γ Q ι) : sentence Γ (Q ⊕ R) ι := σ.map_q sum.inl (by { intros _ _ _ _ _ h, unfold halt start, simp[σ.proper h] })
+instance : has_Sup (sentence Γ Q ι) := ⟨λ s, 
+{ carrier := ⋃₀ (carrier '' s),
+  proper' := λ c z u q x h, by { simp at h, rcases h with ⟨σ, _, hσ⟩, exact σ.proper hσ } }⟩
 
-def dsum_sumr (τ : sentence Γ R ι) : sentence Γ (Q ⊕ R) ι := τ.map_q sum.inr (by { intros _ _ _ _ _ h, unfold halt start, simp[τ.proper h] })
+lemma Sup_carrier (s : set (sentence Γ Q ι)) : ↑(Sup s) = ⋃₀ (carrier '' s) := by refl
 
-def dsum (σ : sentence Γ Q ι) (τ : sentence Γ R ι) : sentence Γ (Q ⊕ R) ι :=
+lemma coe_supr {α : Sort*} {f : α → sentence Γ Q ι} : (↑(⨆ i, f i) : set (word Γ Q ι)) = ⋃ i, (f i) :=
+by { unfold supr, rw [Sup_carrier], simp, refl }
+
+def deterministic.Sup {s : set (sentence Γ Q ι)} (d : ∀ σ ∈ s, deterministic σ) 
+  (h : ∀ (σ ∈ s) (τ ∈ s) {q x c₁ c₂ z₁ z₂ u₁ u₂},
+    ⟮c₁, z₁; u₁ | q, x⟯ ∈ σ → ⟮c₂, z₂; u₂ | q, x⟯ ∈ τ → c₁ = c₂ ∧ z₁ = z₂ ∧ u₁ = u₂) :
+  deterministic (Sup s) :=
+begin
+  rintros q x c₁ c₂ z₁ z₂ u₁ u₂ ⟨_, ⟨σ, hσs, rfl⟩, hσ⟩ ⟨_, ⟨τ, hτs, rfl⟩, hτ⟩, 
+  refine h _ hσs _ hτs hσ hτ
+end
+
+def comp_suml (σ : sentence Γ Q ι) : sentence Γ (Q ⊕ R) ι := σ.map_q sum.inl (by { intros _ _ _ _ _ h, unfold halt start, simp[σ.proper h] })
+
+def comp_sumr (τ : sentence Γ R ι) : sentence Γ (Q ⊕ R) ι := τ.map_q sum.inr (by { intros _ _ _ _ _ h, unfold halt start, simp[τ.proper h] })
+
+def comp (σ : sentence Γ Q ι) (τ : sentence Γ R ι) : sentence Γ (Q ⊕ R) ι :=
 (σ.map_q sum.inl (by { intros _ _ _ _ _ h, unfold halt start, simp[σ.proper h] })) ∪
 (τ.map_q sum.inr (by { intros _ _ _ _ _ h, unfold halt start, simp[τ.proper h] })) ∪
 (fix_q (sum.inl (halt : Q)) (sum.inr (start : R)) (by unfold halt start; simp))
 
-infix ` ⨁ `:80 := dsum
+infix ` ▷ `:80 := comp
 
-lemma dsum.deterministic {σ : sentence Γ Q ι} {τ : sentence Γ R ι}
-  (d₁ : deterministic σ) (d₂ : deterministic τ) : deterministic (σ ⨁ τ) :=
+lemma comp.deterministic {σ : sentence Γ Q ι} {τ : sentence Γ R ι}
+  (d₁ : deterministic σ) (d₂ : deterministic τ) : deterministic (σ ▷ τ) :=
 begin
   refine (deterministic.union (deterministic.union (deterministic.map_q sum.inl_injective d₁) (deterministic.map_q sum.inr_injective d₂) _)
            (fix_q.deterministic _ _ _) _),
@@ -392,56 +489,299 @@ begin
     { simp at eqn, contradiction } }
 end
 
+def dsum (σ : sentence Γ Q ι) (τ : sentence Γ R ι) (c : Q → R → Prop) : sentence Γ (Q ⊕ R) ι :=
+(σ.map_q sum.inl (by { intros _ _ _ _ _ h, unfold halt start, simp[σ.proper h] })) ∪
+(τ.map_q sum.inr (by { intros _ _ _ _ _ h, unfold halt start, simp[τ.proper h] })) ∪
+(⨆ (q : Q) (r : R) (h : c q r), (fix_q (sum.inl q) (sum.inr r) (by unfold halt start; simp)))
+
+lemma dsum.deterministic {σ : sentence Γ Q ι} {τ : sentence Γ R ι}
+  (d₁ : deterministic σ) (d₂ : deterministic τ) (c : Q → R → Prop)
+  (dc : ∀ q r₁ r₂, c q r₁ → c q r₂ → r₁ = r₂)
+  (hc : ∀ q r, c q r → σ.is_halt q) : deterministic (dsum σ τ c) :=
+begin
+  refine (deterministic.union
+    (deterministic.union (deterministic.map_q sum.inl_injective d₁) (deterministic.map_q sum.inr_injective d₂) _)
+      (deterministic.Sup _ _) _),
+  { rintros (q | r) _ _ _ _ _ _ _ ⟨⟨c₁, z₁, u₁, q, x⟩, mem₁, eqn₁⟩ ⟨⟨c₂, z₂, u₂, q', x'⟩, mem₂, eqn₂⟩,
+    { simp at eqn₂, contradiction },
+    { simp at eqn₁, contradiction } },
+  { rintros σ ⟨q, rfl⟩, show (⨆ r (h : c q r), fix_q (sum.inl q) (sum.inr r) _).deterministic,
+    refine deterministic.Sup _ _,
+    { rintros _ ⟨r, rfl⟩, refine deterministic.Sup (by simpa using λ _, fix_q.deterministic _ _ _) _,
+      { rintros _ ⟨_, rfl⟩ _ ⟨_, rfl⟩ (q | r); { intros _ _ _ _ _ _ _ h₁ h₂, exact fix_q.deterministic _ _ _ h₁ h₂ } } },
+    { rintros _ ⟨r₁, rfl⟩ _ ⟨r₂, rfl⟩ (q' | r');
+      { rintros _ _ _ _ _ _ _ ⟨_, ⟨_, ⟨hc₁, rfl⟩, rfl⟩, h₁⟩ ⟨_, ⟨_, ⟨hc₂, rfl⟩, rfl⟩, h₂⟩,
+        have : r₁ = r₂, from dc _ _ _ hc₁ hc₂, rcases this with rfl,
+        exact fix_q.deterministic _ _ (by unfold halt start; simp) h₁ h₂ } } },
+  { rintros _ ⟨q₁, rfl⟩ _ ⟨q₂, rfl⟩ (q | r),
+    { rintros _ _ _ _ _ _ _
+        ⟨_, ⟨_, ⟨r₁, rfl⟩, rfl⟩, ⟨_, ⟨_, ⟨hc₁, rfl⟩, rfl⟩, h₁⟩⟩
+        ⟨_, ⟨_, ⟨r₂, rfl⟩, rfl⟩, ⟨_, ⟨_, ⟨hc₂, rfl⟩, rfl⟩, h₂⟩⟩,
+      simp at h₁ h₂,
+      have : c₁ = sum.inr r₁ ∧ z₁ = x ∧ q = q₁ ∧ u₁ = instruction.Stay,
+      { simpa using fix_q_mem_iff.mp h₁, unfold halt start; simp },
+      rcases this with ⟨rfl, rfl, rfl, rfl⟩,
+      have : c₂ = sum.inr r₂ ∧ z₂ = z₁ ∧ q = q₂ ∧ u₂ = instruction.Stay,
+      { simpa using fix_q_mem_iff.mp h₂, unfold halt start; simp },
+      rcases this with ⟨rfl, rfl, rfl, rfl⟩,
+      have : r₁ = r₂, from dc _ _ _ hc₁ hc₂, rcases this with rfl,
+      simp },
+    { simp,  rintros _ _ _ _ _ _ _
+        ⟨_, ⟨_, ⟨r₁, rfl⟩, rfl⟩, ⟨_, ⟨_, ⟨hc₁, rfl⟩, rfl⟩, h₁⟩⟩ _,
+      have : false, { simpa using (fix_q_mem_iff.mp h₁), unfold start halt; simp },
+      contradiction } },
+  { rintros (q | r),
+    { rintros x _ _ _ _ _ _ (⟨⟨c₁, z₁, u₁, q₁, x₁⟩, wmem, hw⟩ | ⟨⟨c₁, z₁, u₁, q₁, x₁⟩, wmem, hw⟩),
+      { simp at hw, rcases hw with ⟨rfl, rfl, rfl, rfl, rfl⟩,
+        rintros ⟨_, ⟨_, ⟨q', rfl⟩, rfl⟩, ⟨_, ⟨_, ⟨r', rfl⟩, rfl⟩, H, ⟨_, ⟨hc', rfl⟩, rfl⟩, h₁⟩⟩,
+        have : q₁ = q',
+        { have := fix_q_mem_iff.mp h₁, simp at this, rcases this with ⟨rfl, rfl, rfl, rfl⟩; refl,
+          unfold start halt; simp },
+        rcases this with rfl,
+        have : false := hc _ _ hc' wmem, contradiction },
+      { simp at hw, contradiction } },
+    { rintros x _ _ _ _ _ _ (⟨⟨c₁, z₁, u₁, q₁, x₁⟩, wmem, hw⟩ | ⟨⟨c₁, z₁, u₁, q₁, x₁⟩, wmem, hw⟩), 
+      { simp at hw, contradiction },
+      { simp at hw, rcases hw with ⟨rfl, rfl, rfl, rfl, rfl⟩,
+        rintros ⟨_, ⟨_, ⟨q', rfl⟩, rfl⟩, ⟨_, ⟨_, ⟨r', rfl⟩, rfl⟩, H, ⟨_, ⟨hc', rfl⟩, rfl⟩, h₁⟩⟩,
+        have : false, { have := fix_q_mem_iff.mp h₁, simpa using this, unfold start halt; simp },
+        contradiction } } }
+end
+
 end sentence
 
-lemma time_reductions.dsum_aux  {σ : sentence Γ Q ι} {τ : sentence Γ R ι} {n₁ n₂} {q r T₁ T₂ T₃ H₁ H₂ H₃}
+lemma time_reductions.comp_aux {σ : sentence Γ Q ι} {τ : sentence Γ R ι} {n₁ n₂} {q r T₁ T₂ T₃ H₁ H₂ H₃}
   (h₁ : ⟦q, T₁, H₁⟧ ⟶^(n₁)[σ] ⟦halt, T₂, H₂⟧) (h₂ : ⟦start, T₂, H₂⟧ ⟶^(n₂)[τ] ⟦r, T₃, H₃⟧) :
-  ⟦sum.inl q, T₁, H₁⟧ ⟶^(n₁ + n₂ + 1)[σ ⨁ τ] ⟦sum.inr r, T₃, H₃⟧ :=
+  ⟦sum.inl q, T₁, H₁⟧ ⟶^(n₁ + n₂ + 1)[σ ▷ τ] ⟦sum.inr r, T₃, H₃⟧ :=
 begin
-  have h₁ : ⟦sum.inl q, T₁, H₁⟧ ⟶^(n₁)[σ ⨁ τ] ⟦sum.inl halt, T₂, H₂⟧,
+  have h₁ : ⟦sum.inl q, T₁, H₁⟧ ⟶^(n₁)[σ ▷ τ] ⟦sum.inl halt, T₂, H₂⟧,
   from time_reductions.of_ss (time_reductions.map_q sum.inl h₁)
-    (by { simp[(⨁)], refine set.subset_union_of_subset_left (set.subset_union_left _ _) _,
+    (by { simp[(▷)], refine set.subset_union_of_subset_left (set.subset_union_left _ _) _,
           { intros _ _ _ _ _ h, unfold halt start, simp[σ.proper h] } }),
-  have h : ⟦sum.inl halt, T₂, H₂⟧ ⟶¹[σ ⨁ τ] ⟦sum.inr start, T₂, H₂⟧,
+  have h : ⟦sum.inl halt, T₂, H₂⟧ ⟶¹[σ ▷ τ] ⟦sum.inr start, T₂, H₂⟧,
   from reduction.of_ss (sentence.fix_q_reduction _ _ _ _ _)
-    (by { simp[(⨁)], refine set.subset_union_right _ _, { unfold halt start; simp } }),
-  have h₂ : ⟦sum.inr start, T₂, H₂⟧ ⟶^(n₂)[σ ⨁ τ] ⟦sum.inr r, T₃, H₃⟧,
+    (by { simp[(▷)], refine set.subset_union_right _ _, { unfold halt start; simp } }),
+  have h₂ : ⟦sum.inr start, T₂, H₂⟧ ⟶^(n₂)[σ ▷ τ] ⟦sum.inr r, T₃, H₃⟧,
   from time_reductions.of_ss (time_reductions.map_q sum.inr h₂)
-    (by { simp[(⨁)], refine set.subset_union_of_subset_left (set.subset_union_right _ _) _,
+    (by { simp[(▷)], refine set.subset_union_of_subset_left (set.subset_union_right _ _) _,
           { intros _ _ _ _ _ h, unfold halt start, simp[τ.proper h] } }),
   simpa[show n₁.succ + n₂ = n₁ + n₂ + 1, by omega] using (h₁.succ h).add h₂
 end
 
-lemma time_reductions.dsum  {σ : sentence Γ Q ι} {τ : sentence Γ R ι} {n₁ n₂ : ℕ} {T₁ T₂ T₃ H₁ H₂ H₃}
+lemma time_reductions.comp {σ : sentence Γ Q ι} {τ : sentence Γ R ι} {n₁ n₂ : ℕ} {T₁ T₂ T₃ H₁ H₂ H₃}
   (h₁ : ⟦start, T₁, H₁⟧ ⟶^(n₁)[σ] ⟦halt, T₂, H₂⟧) (h₂ : ⟦start, T₂, H₂⟧ ⟶^(n₂)[τ] ⟦halt, T₃, H₃⟧) :
-  ⟦start,  T₁, H₁⟧ ⟶^(n₁ + n₂ + 1)[σ ⨁ τ] ⟦halt, T₃, H₃⟧ :=
-time_reductions.dsum_aux h₁ h₂
+  ⟦start,  T₁, H₁⟧ ⟶^(n₁ + n₂ + 1)[σ ▷ τ] ⟦halt, T₃, H₃⟧ :=
+time_reductions.comp_aux h₁ h₂
 
-lemma time_bounded_reductions.dsum  {σ : sentence Γ Q ι} {τ : sentence Γ R ι} {k₁ k₂ : ℕ} {T₁ T₂ T₃ H₁ H₂ H₃}
+lemma time_bounded_reductions.comp {σ : sentence Γ Q ι} {τ : sentence Γ R ι} {k₁ k₂ : ℕ} {T₁ T₂ T₃ H₁ H₂ H₃}
   (h₁ : ⟦start, T₁, H₁⟧ ⟶^(≤ k₁)[σ] ⟦halt, T₂, H₂⟧) (h₂ : ⟦start, T₂, H₂⟧ ⟶^(≤ k₂)[τ] ⟦halt, T₃, H₃⟧) :
-  ⟦start,  T₁, H₁⟧ ⟶^(≤ k₁ + k₂ + 1)[σ ⨁ τ] ⟦halt, T₃, H₃⟧ :=
-by { rcases h₁ with ⟨n₁, le₁, h₁⟩, rcases h₂ with ⟨n₂, le₂, h₂⟩, refine ⟨n₁ + n₂ + 1, by linarith, time_reductions.dsum h₁ h₂⟩ }
+  ⟦start,  T₁, H₁⟧ ⟶^(≤ k₁ + k₂ + 1)[σ ▷ τ] ⟦halt, T₃, H₃⟧ :=
+by { rcases h₁ with ⟨n₁, le₁, h₁⟩, rcases h₂ with ⟨n₂, le₂, h₂⟩, refine ⟨n₁ + n₂ + 1, by linarith, time_reductions.comp h₁ h₂⟩ }
 
+lemma time_reductions.dsum_left {σ : sentence Γ Q ι} {τ : sentence Γ R ι} {q₁ q₂ T₁ T₂ H₁ H₂} {n}
+  (h : ⟦q₁, T₁, H₁⟧ ⟶^(n)[σ] ⟦q₂, T₂, H₂⟧) (φ : Q → R → Prop) :
+  ⟦sum.inl q₁, T₁, H₁⟧ ⟶^(n)[sentence.dsum σ τ φ] ⟦sum.inl q₂, T₂, H₂⟧ :=
+by exact time_reductions.of_ss (time_reductions.map_q sum.inl h)
+    (by { simp, refine set.subset_union_of_subset_left (set.subset_union_left _ _) _,
+          { intros _ _ _ _ _ h, unfold halt start, simp[σ.proper h] } })
+
+lemma time_reductions.dsum_right {σ : sentence Γ Q ι} {τ : sentence Γ R ι} {r₁ r₂ T₁ T₂ H₁ H₂} {n}
+  (h : ⟦r₁, T₁, H₁⟧ ⟶^(n)[τ] ⟦r₂, T₂, H₂⟧) (φ : Q → R → Prop) :
+  ⟦sum.inr r₁, T₁, H₁⟧ ⟶^(n)[sentence.dsum σ τ φ] ⟦sum.inr r₂, T₂, H₂⟧ :=
+by exact time_reductions.of_ss (time_reductions.map_q sum.inr h)
+    (by { simp, refine set.subset_union_of_subset_left (set.subset_union_right _ _) _,
+          { intros _ _ _ _ _ h, unfold halt start, simp[τ.proper h] } })
+
+lemma time_reductions.dsum {σ : sentence Γ Q ι} {τ : sentence Γ R ι} {n₁ n₂} {q₁ q₂ r₂ r₃ T₁ T₂ T₃ H₁ H₂ H₃}
+  (φ : Q → R → Prop) (h : φ q₂ r₂)
+  (h₁ : ⟦q₁, T₁, H₁⟧ ⟶^(n₁)[σ] ⟦q₂, T₂, H₂⟧) (h₂ : ⟦r₂, T₂, H₂⟧ ⟶^(n₂)[τ] ⟦r₃, T₃, H₃⟧) :
+  ⟦sum.inl q₁, T₁, H₁⟧ ⟶^(n₁ + n₂ + 1)[sentence.dsum σ τ φ] ⟦sum.inr r₃, T₃, H₃⟧ :=
+begin
+  have h₁ : ⟦sum.inl q₁, T₁, H₁⟧ ⟶^(n₁)[sentence.dsum σ τ φ] ⟦sum.inl q₂, T₂, H₂⟧,
+  from time_reductions.dsum_left h₁ φ,
+  have h : ⟦sum.inl q₂, T₂, H₂⟧ ⟶¹[sentence.dsum σ τ φ] ⟦sum.inr r₂, T₂, H₂⟧,
+  from reduction.of_ss (sentence.fix_q_reduction _ _ _ _ _)
+    (by { refine set.subset_union_of_subset_right _ _, { unfold halt start; simp },
+      simp[sentence.coe_supr], refine set.subset_Union₃ q₂ r₂ h }),
+  have h₂ : ⟦sum.inr r₂, T₂, H₂⟧ ⟶^(n₂)[sentence.dsum σ τ φ] ⟦sum.inr r₃, T₃, H₃⟧,
+  from time_reductions.dsum_right h₂ φ,
+  simpa[show n₁.succ + n₂ = n₁ + n₂ + 1, by omega] using (h₁.succ h).add h₂
+end
+
+lemma time_bounded_reductions.dsum {σ : sentence Γ Q ι} {τ : sentence Γ R ι} {n₁ n₂} {q₁ q₂ r₂ r₃ T₁ T₂ T₃ H₁ H₂ H₃}
+  (φ : Q → R → Prop) (h : φ q₂ r₂)
+  (h₁ : ⟦q₁, T₁, H₁⟧ ⟶^(≤ n₁)[σ] ⟦q₂, T₂, H₂⟧) (h₂ : ⟦r₂, T₂, H₂⟧ ⟶^(≤ n₂)[τ] ⟦r₃, T₃, H₃⟧) :
+  ⟦sum.inl q₁, T₁, H₁⟧ ⟶^(≤ n₁ + n₂ + 1)[sentence.dsum σ τ φ] ⟦sum.inr r₃, T₃, H₃⟧ :=
+by{ rcases h₁ with ⟨n₁, le₁, h₁⟩, rcases h₂ with ⟨n₂, le₂, h₂⟩,
+    refine ⟨n₁ + n₂ + 1, by linarith, time_reductions.dsum φ h h₁ h₂⟩ }
 
 end model
-/--/
-namespace sentence
 
-namespace delete
+namespace blang
+open instruction model
+variables (Γ Q ι) [inhabited Γ] [bfin Γ]
 
-inductive srh
-| start
-| run
-| halt
+def list_less_than (k : ℕ) := {l : list (option bool) // l.length ≤ k}
 
-instance : state_lang srh := ⟨srh.start, srh.halt⟩
+instance (k : ℕ) : inhabited (list_less_than k) := ⟨⟨[], by simp⟩⟩
 
-inductive main (i : fin ι) : sentence (language Γ) srh ι
-| start : ∀ v, main (⟨start, v⟩ ▷ ⟨srh.run, ⟩)
-| halt : main (⟨srh.run, vector.repeat ␤ ι⟩ ▷ ⟨halt, vector.repeat (␤, instruction.stay) ι⟩)
+namespace read
 
-end delete
+inductive state
+| intro (q : Q) (i : fin (bentropy Γ).succ) (v : vector (vector bool (bentropy Γ)) ι) : state
 
-end sentence
+variables {Γ Q ι}
+
+instance [state_lang Q] : state_lang (state Γ Q ι) :=
+⟨state.intro start 0 default, state.intro halt ⊤ default⟩
+
+def δ : state Γ Q ι → vector bool ι → option (state Γ Q ι × vector bool ι × vector instruction ι)
+| ⟨q, i, v⟩ x := if h : i < ⊤ then 
+    let newstate : state Γ Q ι :=
+      ⟨q, ⟨i + 1, nat.succ_lt_succ (fin.lt_top_iff.mp h)⟩, (v.sim_update_nth (vector.rep ⟨i, fin.lt_top_iff.mp h⟩) x)⟩ in 
+  some ⟨newstate, x, Right⟩ else none
+
+@[simp] lemma δ_top {q v x} : δ (⟨q, ⊤, v⟩ : state Γ Q ι) x = none := by simp[δ]
+
+def σ : sentence bool (state Γ Q ι) ι := sentence.of_fun δ
+(by { unfold start halt,
+      intros q x c z u eqn, split; rintros rfl,
+      { simpa using eqn },
+      { rcases q with ⟨q, i, v⟩, by_cases C : i < ⊤; simp[C, δ, fin.ext_iff] at eqn; contradiction } })
+
+section
+variables (v : vector (vector bool (bentropy Γ)) ι) (T : vector (ℕ → bool) ι) (H : vector ℕ ι)
+
+lemma σ_reduction (q : Q) (i : fin (bentropy Γ).succ) (h : i < ⊤) :
+  ⟦⟨q, i, v⟩, T, H⟧ ⟶¹[σ]
+  ⟦⟨q, ⟨i + 1, nat.succ_lt_succ (fin.lt_top_iff.mp h)⟩, 
+    v.sim_update_nth (vector.rep ⟨i, fin.lt_top_iff.mp h⟩) (read T H)⟩, T, H.map nat.succ⟧ :=
+reduction.iff.mpr (⟨read T H, Right, by simp[σ, δ, h], by simp, by ext; simp⟩)
+
+@[simp] lemma σ_is_halt (q : Q) (v : vector (vector bool (bentropy Γ)) ι) : σ.is_halt ⟨q, ⊤, v⟩ :=
+by intros c z u x; simp[σ]
+
+def memory :
+  fin (bentropy Γ).succ → vector (vector bool (bentropy Γ)) ι
+| ⟨0, _⟩      := v
+| ⟨s + 1, hn⟩ := (memory ⟨s, by omega⟩).sim_update_nth (vector.rep ⟨s, by omega⟩) (read T (H.map ((+) s)))
+
+@[simp] lemma memory_0 : memory v T H 0 = v := by unfold has_zero.zero; rw [memory]
+
+lemma σ_time_reductions (q : Q) :
+  ∀ (s : fin (bentropy Γ).succ), ⟦⟨q, 0, v⟩, T, H⟧ ⟶^(s)[σ] ⟦⟨q, s, memory v T H s⟩, T, H.map ((+) s)⟧
+| ⟨0, _⟩      := by { simp, ext, simp, }
+| ⟨s + 1, hs⟩ := by { 
+    let s' : fin (bentropy Γ).succ := ⟨s, by omega⟩,
+    have r : ⟦⟨q, 0, v⟩, T, H⟧ ⟶^(s)[σ] ⟦⟨q, ⟨s, _⟩, memory v T H ⟨s, _⟩⟩, T, H.map ((+) s)⟧,
+    from σ_time_reductions ⟨s, by omega⟩,
+    have : ⟦⟨q, ⟨s, _⟩, memory v T H ⟨s, _⟩⟩, T, H.map ((+) s)⟧ ⟶¹[σ] ⟦⟨q, ⟨s + 1, _⟩, memory v T H ⟨s + 1, _⟩⟩, T, _⟧,
+    by simpa[memory] using
+      σ_reduction (memory v T H s') T (H.map ((+) s)) q s' (by simp[fin.lt_top_iff]; exact nat.succ_lt_succ_iff.mp hs),
+    rw [show (H.map ((+) s)).map nat.succ = H.map ((+) s.succ), by ext; simp[nat.succ_add]] at this,
+    exact r.succ this }
+
+lemma memory_nth_nth_of_lt : ∀ (s : fin (bentropy Γ).succ) k i (h : ↑i < s), 
+  ((memory v T H s).nth k).nth i = T.nth k (i + H.nth k)
+| ⟨0, _⟩ k i hi := by simp at hi; contradiction
+| ⟨s + 1, hs⟩ k ⟨i, hi⟩ h := by { 
+    have : i = s ∨ i < s, from eq_or_lt_of_le (nat.lt_succ_iff.mp (by simpa using h)),
+    rcases this with (rfl | lt); simp[memory, vector.nth_sim_update_nth_if],
+    { have : s ≠ i, from ne_of_gt lt,
+      simp[this],
+      simpa using memory_nth_nth_of_lt ⟨s, lt_trans (lt_add_one s) hs⟩ k ⟨i, hi⟩ (by simpa using lt) } }
+
+lemma σ_time_reductions_top (q : Q) : ⟦⟨q, 0, v⟩, T, H⟧ ⟶^(bentropy Γ)[σ] ⟦⟨q, ⊤, memory v T H ⊤⟩, T, H.map ((+) (bentropy Γ))⟧ :=
+σ_time_reductions v T H q ⊤
+
+lemma memory_nth_nth (k i) : ((memory v T H ⊤).nth k).nth i = T.nth k (i + H.nth k) :=
+memory_nth_nth_of_lt v T H ⊤ k i (by simp[fin.lt_top_iff]; exact fin.is_lt i)
+
+end
+
+end read
+
+namespace write
+
+inductive state
+| intro (q : Q) (i : fin (bentropy Γ).succ) (v : vector (vector bool (bentropy Γ)) ι) (u : vector instruction ι) : state
+
+variables {Γ Q ι}
+
+instance [state_lang Q] : state_lang (state Γ Q ι) :=
+⟨state.intro start ⊤ default Stay, state.intro halt 0 default Stay⟩
+
+def δ : state Γ Q ι → vector bool ι → option (state Γ Q ι × vector bool ι × vector instruction ι)
+| ⟨q, ⟨0, _⟩, v, u⟩      x := none
+| ⟨q, ⟨i + 1, hi⟩, v, u⟩ x := 
+    let newstate : state Γ Q ι := ⟨q, ⟨i, by omega⟩, v, u⟩,
+        i' : fin (bentropy Γ)  := ⟨i, nat.succ_lt_succ_iff.mp hi⟩ in 
+  some ⟨newstate, v.map (λ x, x.nth i'), Left⟩
+
+@[simp] lemma δ_top {q v x u} : δ (⟨q, 0, v, u⟩ : state Γ Q ι) x = none := by unfold has_zero.zero; rw [δ]
+
+def σ : sentence bool (state Γ Q ι) ι := sentence.of_fun δ
+(by { unfold start halt,
+      intros q x c z u eqn, split; rintros rfl,
+      { simpa using eqn },
+      { rcases q with ⟨q, ⟨i, hi⟩, v, u⟩, rcases i; simp[δ] at eqn,
+        { contradiction },
+        { have lt : i < bentropy Γ, from nat.succ_lt_succ_iff.mp hi,
+          have eq : i = bentropy Γ, by simpa[fin.coe_top] using (fin.eq_iff_veq _ _).mp eqn.1.2.1,
+          simp[eq] at lt, contradiction } } })
+
+section
+variables (v : vector (vector bool (bentropy Γ)) ι) (u : vector instruction ι) (T : vector (ℕ → bool) ι) (H : vector ℕ ι)
+
+def σ_tape_reduct (i) :=
+vector.zip_with3 (λ (t : ℕ → bool) h (x : vector bool (bentropy Γ)) n, if n = h then x.nth i else t n) T H v
+
+lemma σ_reduction (q : Q) (i : ℕ) (hi) :
+  ⟦⟨q, ⟨i + 1, hi⟩, v, u⟩, T, H⟧ ⟶¹[σ]
+  ⟦⟨q, ⟨i, by omega⟩, v, u⟩, σ_tape_reduct v T H ⟨i, nat.succ_lt_succ_iff.mp hi⟩, H.map nat.pred⟧ :=
+reduction.iff.mpr (⟨v.map (λ x, x.nth ⟨i, (by omega)⟩), Left, by simp[σ, δ]; refl,
+  by { simp[reduct_tape, σ_tape_reduct], ext, simp }, by { ext, simp, exact nat.pred_eq_sub_one _ }⟩)
+
+@[simp] lemma σ_is_halt (q : Q) : σ.is_halt ⟨q, 0, v, u⟩ :=
+λ c z u x, by simp[σ]
+
+def Tape : fin (bentropy Γ).succ → vector (vector bool (bentropy Γ)) ι → vector (ℕ → bool) ι → vector ℕ ι → vector (ℕ → bool) ι
+| ⟨0, _⟩      v T H := T
+| ⟨s + 1, hn⟩ v T H := Tape ⟨s, by omega⟩ v (σ_tape_reduct v T H ⟨s, nat.succ_lt_succ_iff.mp hn⟩) (H.map nat.pred)
+
+@[simp] lemma Tape_0 : Tape 0 v T H = T := by unfold has_zero.zero; rw [Tape]
+
+lemma σ_time_reductions (q : Q) :
+  ∀ (s : fin (bentropy Γ).succ) (T H), ⟦⟨q, s, v, u⟩, T, H⟧ ⟶^(s)[σ] ⟦⟨q, 0, v, u⟩, Tape s v T H, (H.map (λ h, h - s))⟧
+| ⟨0, _⟩      T H := by { simp, ext, simp }
+| ⟨s + 1, hs⟩ T H := by { 
+    let s' : fin (bentropy Γ).succ := ⟨s, by omega⟩,
+    let s'' : fin (bentropy Γ) := ⟨s, by { exact nat.succ_lt_succ_iff.mp hs}⟩,
+    have r : ⟦⟨q, ⟨s, _⟩, v, u⟩, _, H.map nat.pred⟧ ⟶^(s)[σ] ⟦⟨q, 0, v, u⟩, _, H.map (λ h, h - (s + 1))⟧,
+    { have := σ_time_reductions ⟨s, by omega⟩ (σ_tape_reduct v T H ⟨s, by omega⟩) (H.map nat.pred), simp at this, 
+      rw[show (H.map nat.pred).map (λ h, h - s) = H.map (λ h, h - (s + 1)),
+         by { ext; simp;  rw[nat.pred_sub, nat.pred_eq_sub_one, tsub_tsub] }] at this,
+      exact this },
+    have : ⟦⟨q, ⟨s + 1, _⟩, v, u⟩, T, H⟧ ⟶¹[σ] ⟦⟨q, ⟨s, _⟩, v, u⟩, _, H.map nat.pred⟧,
+    from σ_reduction v u T H q s hs,
+    have : ⟦⟨q, ⟨s + 1, _⟩, v, u⟩, T, H⟧ ⟶^(s+1)[σ] ⟦⟨q, 0, v, u⟩, _, H.map (λ h, h - (s + 1))⟧,
+    from relation.power.succ_inv this r,
+    simpa[Tape, @sub_add_eq_sub_sub ℕ] using this }
+
+end
+
+end write
+
+end blang
+
+
+namespace universal_tm
+variables {Γ Q ι}
+
+abbreviation lang := word Γ Q ι ⊕ vector Γ ι
+
+
+
+end universal_tm
 
 end turing_machine
